

Discrete Structure Assignment 1 (Section 02)

Group members: Cheng Zhi Min A25CS0050

Gan Mei Lee A25CS0225

Ng Xuan Yee A25CS0291

$$1. (a) x^2 + x - 6 = 0$$

$$(x-2)(x+3) = 0$$

$$x = -3, x = 2$$

$$A = \{-3, 2\}$$

$$\therefore A' = \{x \in \mathbb{Z} \mid x \neq -3, x \neq 2\}$$

$$(b) (B-A) \cap C = \{1, 4\} \cap \{2, 3, 4\}$$

$$= \{4\}$$

$$1. (c) B \cap C = \{2, 4\}$$

$$n = 2$$

$$|P(B \cap C)| = 2^n = 2^2 = 4$$

$$2. (((P \vee Q) \wedge R)' \vee Q')' = (((P \vee Q) \wedge R)')' \wedge (Q')' \rightarrow \text{De Morgan's Law}$$

$$= ((P \vee Q) \wedge R) \wedge Q \rightarrow \text{Double Complement Law}$$

$$= Q \wedge ((P \vee Q) \wedge R) \rightarrow \text{Commutative Law}$$

$$= (Q \wedge (P \vee Q)) \wedge R \rightarrow \text{Associative Law}$$

$$= Q \wedge R \rightarrow \text{Absorption Law}$$

3. (a) $|A|$ = number of students in art class.
 $|S|$ = number of students in science class.

$$|A \cup S| = |A| + |S| - |A \cap S|$$

$$= 35 + 57 - 12$$

$$= 80$$

\therefore 80 students

$$(b) |A \cup S| = |A| + |S| - |A \cap S|$$

$$= 35 + 57 - 0$$

$$= 92$$

\therefore 92 students.

4. (a) p : you try hard
 q : you have a talent
 r : you will get rich
 $\therefore (p \wedge q) \rightarrow r$

(b) The statement false implies that r must be false and $(p \wedge q)$ must be true, because a statement $X \rightarrow Y$ is false when X is true and Y is false. Since p is true (you try hard) and r is false, then q must be true as

$$(p \wedge q) \rightarrow r = (T \wedge T) \rightarrow F = T \rightarrow F = F.$$

\therefore You try hard and have a talent but you do not get rich.

(c) r is true (you are rich). Since r is true, the statement $(p \wedge q) \rightarrow r$ must be true, because an $X \rightarrow Y$ statement is true whenever Y is true.
 \therefore The statement is true.

5.

P	q	r	$r \rightarrow p$	$q \wedge (r \rightarrow p)$	$p \vee (q \wedge (r \rightarrow p))$	A	$\sim p$	$q \rightarrow r$	B
F	F	F	T	F	F	T	T	T	T
F	F	T	F	F	F	T	T	T	T
F	T	F	T	T	T	F	T	F	F
F	T	T	F	F	F	T	T	T	T
T	F	F	T	F	T	F	F	T	F
T	F	T	T	F	T	F	F	T	F
T	T	F	T	T	T	F	F	F	F
T	T	T	T	T	T	F	F	T	F

$\therefore A \equiv B$.

6. Assume x is odd and y is even.

Since x is odd, $x = 2h + 1$ for some integer h , and since y is even, $y = 2k$ for some integer k .

$$x^2 - 2y = (2h + 1)^2 - 2(2k)$$

$$= 4h^2 + 4h + 1 - 4k$$

$$= 2(2h^2 + 2h - 2k) + 1$$

$$= 2r + 1, \text{ where } r = 2h^2 + 2h - 2k \text{ for some integer } r.$$

\therefore since $x^2 - 2y$ satisfies the form of $2(\text{integer}) + 1$, therefore $x^2 - 2y$ is odd. The statement is true and is proven.